adding sorts

template-coq/theories/Universes.v
@@ -1,7 +1,8 @@
 From Coq Require Import MSetList MSetFacts MSetProperties MSetDecide.
+From Coq Require Import Structures.OrdersEx.
 From MetaCoq.Template Require Import utils BasicAst config.
 From Equations Require Import Equations.
-Require Import ssreflect.
+Require Import ssreflect ssrbool.
 
 Local Open Scope nat_scope.
 Local Open Scope string_scope2.
@@ -14,29 +15,171 @@ Ltac absurd :=
 Hint Extern 10 => absurd : core.
 (** * Valuations *)
 
-(** A valuation is a universe level (nat) given for each
-    universe variable (Level.t).
+Inductive universe_family :=
+  | UProp
+  | USProp
+  | UType
+  | UGlobal (_ : string) (* name of a global sort *).
+Derive NoConfusion EqDec for universe_family.
+
+(** A valuation is a universe level (nat) given for each universe variable
+    (Level.t) and a sort family (universe_family) for each sort variables.
     It is >= for polymorphic universes and > 0 for monomorphic universes. *)
 Record valuation :=
   { valuation_mono : string -> positive ;
-    valuation_poly : nat -> nat }.
+    valuation_poly : nat -> nat ;
+    valuation_sort : nat -> universe_family }.
 
-Inductive universes := 
-  | UProp 
-  | USProp
-  | UType (i : nat).
-Derive NoConfusion EqDec for universes.
+Definition universes : Type := universe_family * nat.
 
 Class Evaluable (A : Type) := val : valuation -> A -> nat.
 
 (** This inductive classifies which eliminations are allowed for inductive types
   in various sorts. *)
+(* KM: will be managed by universe family constraints instead *)
 Inductive allowed_eliminations : Set :=
 | IntoSProp
 | IntoPropSProp
 | IntoSetPropSProp
 | IntoAny.
 Derive NoConfusion EqDec for allowed_eliminations.
+
+(** * Sorts *)
+
+
+Module SortFamily.
+
+  (* Putting both Prop and SProp for simplifying the modification
+     Consider replacing Prop by an impredicative sort and defining
+     Prop as a global sort above this impredicative sort.
+     (SProp does have some specific handling in conversion so it
+     might be better to keep it)
+   *)
+  Inductive t_ :=
+  | sfProp
+  | sfSProp
+  | sfType
+  | sfGlobal (_ : string) (* name of a global sort *)
+  | sfVar (_ : nat)(* these are debruijn indices *).
+  Derive NoConfusion EqDec for t_.
+
+  Definition t := t_.
+
+  Inductive lt_ : t -> t -> Prop :=
+  | ltSFTypeProp : lt_ sfType sfProp
+  | ltSFTypeSProp : lt_ sfType sfSProp
+  | ltSFTypeGlobal (s : string) : lt_ sfType (sfGlobal s)
+  | ltSFTypeVar (n : nat) : lt_ sfType (sfVar n)
+  | ltSFPropSProp : lt_ sfProp sfSProp
+  | ltSFPropGlobal (s : string) : lt_ sfProp (sfGlobal s)
+  | ltSFPropVar (n : nat) : lt_ sfProp (sfVar n)
+  | ltSFSPropGlobal (s : string) : lt_ sfSProp (sfGlobal s)
+  | ltSFSPropVar (n : nat) : lt_ sfSProp (sfVar n)
+  | ltSFGlobalGlobal (s1 s2 : string) : string_lt s1 s2 -> lt_ (sfGlobal s1) (sfGlobal s2)
+  | ltSFGlobalVar (s: string) (n : nat) : lt_ (sfGlobal s) (sfVar n)
+  | ltSFVarVar (n1 n2 : nat) : Nat.lt n1 n2 -> lt_ (sfVar n1) (sfVar n2).
+
+  Definition lt := lt_.
+
+  Lemma lt_strorder : StrictOrder lt.
+  Proof.
+    constructor.
+    - intros []; intro X; inversion X.
+      1: eapply string_lt_irreflexive; tea.
+      eapply Nat.lt_irrefl; tea.
+    - intros ? ? ? X Y; invs X; invs Y; constructor.
+      1: eapply transitive_string_lt; tea.
+      etransitivity; tea.
+  Qed.
+
+  Lemma lt_compat : Proper (eq ==> eq ==> iff) lt.
+  Proof. move=> ? ? -> ? ? -> //. Qed.
+
+  Definition compare (sf1 sf2 : t) : comparison :=
+    match sf1, sf2 with
+    | sfType, sfType => Eq
+    | sfType, _ => Lt
+    | _, sfType => Gt
+    | sfProp, sfProp => Eq
+    | sfProp, _ => Lt
+    | _, sfProp => Gt
+    | sfSProp, sfSProp => Eq
+    | sfSProp, _ => Lt
+    | _, sfSProp => Gt
+    | sfGlobal s1, sfGlobal s2 => string_compare s1 s2
+    | sfGlobal _, _ => Lt
+    | _, sfGlobal _ => Gt
+    | sfVar n1, sfVar n2 => Nat.compare n1 n2
+    end.
+
+
+  Definition compare_spec :
+    forall x y : t, CompareSpec (x = y) (lt x y) (lt y x) (compare x y).
+  Proof.
+    move=> [| | |s|n] [| | |s'|n']; repeat constructor; cbn.
+    - eapply CompareSpec_Proper.
+      5: eapply CompareSpec_string. 4: reflexivity.
+      all: split; [now inversion 1|]. now intros ->.
+      all: intro; now constructor.
+    - eapply CompareSpec_Proper.
+      5: eapply Nat.compare_spec. 4: reflexivity.
+      all: split; [now inversion 1|]. now intros ->.
+      all: intro; now constructor.
+  Qed.
+
+  Definition eq : t -> t -> Prop := eq.
+  Definition eq_equiv : Equivalence eq := _.
+
+  Definition eq_dec (l1 l2 : t) : {l1 = l2}+{l1 <> l2}.
+  Proof.
+    decide equality. apply string_dec. apply Peano_dec.eq_nat_dec.
+  Defined.
+
+  Definition eqb (sf1 sf2 : t) : bool
+    := match compare sf1 sf2 with Eq => true | _ => false end.
+
+  Global Instance eqb_refl : Reflexive eqb.
+  Proof.
+    intros []; unfold eqb; cbnr.
+    - rewrite (ssreflect.iffRL (string_compare_eq s s)). all: auto.
+    - rewrite Nat.compare_refl. reflexivity.
+  Qed.
+
+  Lemma eqb_spec l l' : reflect (eq l l') (eqb l l').
+  Proof.
+    destruct l, l'; cbn; try constructor; try reflexivity; try discriminate.
+    - apply iff_reflect. unfold eqb; cbn.
+      destruct (CompareSpec_string s s0); split; intro HH;
+        try reflexivity; try discriminate; try congruence.
+      all: inversion HH; subst; now apply string_lt_irreflexive in H.
+    - apply iff_reflect. unfold eqb; cbn.
+      destruct (Nat.compare_spec n n0); split; intro HH;
+        try reflexivity; try discriminate; try congruence.
+      all: inversion HH; subst; now apply Nat.lt_irrefl in H.
+  Qed.
+
+  Definition eq_leibniz (x y : t) : eq x y -> x = y := id.
+
+  Definition is_impredicative (sf : t) : bool :=
+    match sf with
+    | sfProp | sfSProp => true
+    | _ => false
+    end.
+
+
+  Definition sort_val v (x : t) : universe_family :=
+    match x with
+    | sfProp => UProp
+    | sfSProp => USProp
+    | sfType => UType
+    | sfGlobal s => UGlobal s
+    | sfVar k => valuation_sort v k
+    end.
+
+End SortFamily.
+
+
+(** * Level expressions *)
 
 (** Levels are Set or Level or Var *)
 Module Level.
@@ -200,38 +343,6 @@ Proof.
   intros x; rewrite LevelSet.union_spec. lsets.
 Qed.
 
-(* prop level is Prop or SProp *)
-Module PropLevel.
-
-  Inductive t := lSProp | lProp.
-  Derive NoConfusion EqDec for t.
-  (* Global Instance PropLevel_Evaluable : Evaluable t :=
-    fun v l => match l with
-              lSProp => -1
-            | lProp => -1
-            end. *)
-
-  Definition compare (l1 l2 : t) : comparison :=
-    match l1, l2 with
-    | lSProp, lSProp  => Eq
-    | lProp, lProp  => Eq
-    | lProp, lSProp => Gt
-    | lSProp, lProp => Lt
-    end.
-
-  Inductive lt_ : t -> t -> Prop :=
-    ltSPropProp : lt_ lSProp lProp.
-
-  Definition lt := lt_.
-
-  Global Instance lt_strorder : StrictOrder lt.
-  split.
-  - intros n X. destruct n;inversion X.
-  - intros n1 n2 n3 X1 X2. destruct n1,n2,n3;auto; try inversion X1;try inversion X2.
-  Defined.
-
-End PropLevel.
-
 Module UnivExpr.
   (* npe = no prop expression *)
   Definition t := (Level.t * nat)%type.
@@ -342,49 +453,31 @@ Proof.
   - right. intros ->. apply n. reflexivity.
 Qed.
 
-Module Universe.
-  (** A universe is a list of universe expressions which is:
+Module UnivLevel.
+  (** A universe level is a list of universe expressions which is:
         - sorted
         - without duplicate
         - non empty *)
-  Record t0 := { t_set : UnivExprSet.t ;
+  Record t_ := { t_set : UnivExprSet.t ;
                  t_ne  : UnivExprSet.is_empty t_set = false }.
 
-  Derive NoConfusion for t0.
+  Derive NoConfusion for t_.
   
   (** This needs a propositional UIP proof to show that [is_empty = false] is a set *)
   Set Equations With UIP.
-  Instance t0_eqdec : EqDec t0.
-  Proof. eqdec_proof. Qed.
-
-  Inductive t_ :=
-    lProp | lSProp | lType (_ : t0).
-  Derive NoConfusion for t_.
-
   Instance t_eqdec : EqDec t_.
   Proof. eqdec_proof. Qed.
   
+
   Definition t := t_.
 
-  Coercion t_set : t0 >-> UnivExprSet.t.
+  Coercion t_set : t_ >-> UnivExprSet.t.
 
-  Definition eqb (u1 u2 : t) : bool :=
-    match u1, u2 with
-    | lSProp, lSProp => true
-    | lProp, lProp => true
-    | lType e1, lType e2 => UnivExprSet.equal e1.(t_set) e2.(t_set)
-    | _,_ => false
-    end.
+  Definition eqb (x y : t) := UnivExprSet.equal x.(t_set) y.(t_set).
 
-  Definition make' (e : UnivExpr.t) : t0
+  Definition make' (e : UnivExpr.t) : t
     := {| t_set := UnivExprSet.singleton e;
           t_ne := eq_refl |}.
-
-  (** Create a universe representing the given level. *)
-  Definition make (l : Level.t) : t :=
-    lType (make' (UnivExpr.make l)).
-
-  Definition of_expr e := (lType (make' e)).
 
   Lemma not_Empty_is_empty s :
     ~ UnivExprSet.Empty s -> UnivExprSet.is_empty s = false.
@@ -393,7 +486,7 @@ Module Universe.
     apply H. now apply UnivExprSetFact.is_empty_2 in H'.
   Qed.
 
-  Program Definition add (e : UnivExpr.t) (u : t0) : t0
+  Program Definition add (e : UnivExpr.t) (u : t) : t
     := {| t_set := UnivExprSet.add e u |}.
   Next Obligation.
     apply not_Empty_is_empty; intro H.
@@ -401,19 +494,13 @@ Module Universe.
     left; reflexivity.
   Qed.
 
-  Definition add_to_exprs (e : UnivExpr.t) (u : t) : t :=
-    match u with
-    | lSProp |lProp => u
-    | lType l => lType (add e l)
-    end.
-
   Lemma add_spec e u e' :
     UnivExprSet.In e' (add e u) <-> e' = e \/ UnivExprSet.In e' u.
   Proof.
     apply UnivExprSet.add_spec.
   Qed.
 
-  Definition add_list : list UnivExpr.t -> t0 -> t0
+  Definition add_list : list UnivExpr.t -> t -> t
     := List.fold_left (fun u e => add e u).
 
   Lemma add_list_spec l u e :
@@ -436,70 +523,18 @@ Module Universe.
         * apply add_spec; right. apply IHl0. now right.
   Qed.
 
-  Definition add_list_to_exprs (es : list UnivExpr.t) (u : t) : t :=
-    match u with
-    | lSProp |lProp => u
-    | lType l => lType (add_list es l)
-    end.
-
   (** Test if the universe is a lub of levels or contains +n's. *)
   Definition is_levels (u : t) : bool :=
-      match u with
-      | lProp | lSProp => true
-      | lType l =>  UnivExprSet.for_all UnivExpr.is_level l
-      end.
+    UnivExprSet.for_all UnivExpr.is_level u.
 
   (** Test if the universe is a level or an algebraic universe. *)
   Definition is_level (u : t) : bool :=
-    match u with
-    | lProp | lSProp => true
-    | lType l => (UnivExprSet.cardinal l =? 1)%nat && is_levels u
-    end.
-
-  Definition is_sprop (u : t) : bool :=
-    match u with
-      | lSProp => true
-      | _ => false
-    end.
-
-  Definition is_prop (u : t) : bool :=
-    match u with
-      | lProp => true
-      | _ => false
-    end.
-
-  Definition type0 : t := make Level.lSet.
-  Definition type1 : t := lType (make' UnivExpr.type1).
-
-  Definition of_levels (l : PropLevel.t + Level.t) : t :=
-    match l with
-    | inl PropLevel.lSProp => lSProp
-    | inl PropLevel.lProp => lProp
-    | inr l => lType (make' (l, 0%nat))
-    end.
-
-  (* Used for quoting. *)
-  Definition from_kernel_repr (e : Level.t * bool) (es : list (Level.t * bool)) : t
-    := lType (add_list (map UnivExpr.from_kernel_repr es)
-                (make' (UnivExpr.from_kernel_repr e))).
-
-  (* Definition uex_to_kernel_repr (e : UnivExpr.t) : Level.t * bool := *)
-  (*   match e with *)
-  (*   | UnivExpr.npe (l, b) => (NoPropLevel.to_level l, b) *)
-  (*   end. *)
-
-  (* Definition to_kernel_repr (u : t) : list (Level.t * bool) *)
-  (*   :=  map (UnivExpr.to_kernel_repr) (UnivExprSet.elements u). *)
-  (* match u with *)
-  (*      | lProp => [(Level.lProp, false)] *)
-  (*      | lSProp => [(Level.lSProp, false)] *)
-  (*      | lType l => map uex_to_kernel_repr (UnivExprSet.elements l) *)
-  (*      end. *)
+    (UnivExprSet.cardinal u =? 1)%nat && is_levels u.
 
 
   (** The non empty / sorted / without dup list of univ expressions, the
       components of the pair are the head and the tail of the (non empty) list *)
-  Program Definition exprs (u : t0) : UnivExpr.t * list UnivExpr.t
+  Program Definition exprs (u : t) : UnivExpr.t * list UnivExpr.t
     := match UnivExprSet.elements u with
        | [] => False_rect _ _
        | e :: l => (e, l)
@@ -512,15 +547,12 @@ Module Universe.
     rewrite <- Heq_anonymous; reflexivity.
   Qed.
 
-  Lemma exprs_make' e : Universe.exprs (Universe.make' e) = (e, []).
+  Lemma exprs_make' e : exprs (make' e) = (e, []).
   Proof. reflexivity. Defined.
-
-  (* Lemma exprs_make l : Universe.exprs (Universe.make l) = (UnivExpr.make l, []). *)
-  (* Proof. reflexivity. Defined. *)
 
 
   Lemma exprs_spec u :
-    let '(e, u') := Universe.exprs u in
+    let '(e, u') := exprs u in
     e :: u' = UnivExprSet.elements u.
   Proof.
     destruct u as [u1 u2].
@@ -530,7 +562,7 @@ Module Universe.
                 | [] => fun Heq_anonymous : [] = _ u1 =>
                     False_rect (UnivExpr.t × list UnivExpr.t)
                                (exprs_obligation_1
-                                  {| Universe.t_set := u1; Universe.t_ne := u2 |}
+                                  {| t_set := u1; t_ne := u2 |}
                                   Heq_anonymous)
                 | e :: l0 => fun _ : e :: l0 = _ u1 => (e, l0)
                 end eq_refl in e :: u' = UnivExprSet.elements  u1).
@@ -544,32 +576,32 @@ Module Universe.
   Qed.
 
   Lemma exprs_spec' u :
-    (Universe.exprs u).1 :: (Universe.exprs u).2 = UnivExprSet.elements u.
+    (exprs u).1 :: (exprs u).2 = UnivExprSet.elements u.
   Proof.
     pose proof (exprs_spec u).
-    now destruct (Universe.exprs u).
+    now destruct (exprs u).
   Qed.
 
-  Lemma In_exprs (u : t0) (e : UnivExpr.t) :
+  Lemma In_exprs (u : t) (e : UnivExpr.t) :
     UnivExprSet.In e u
-    <-> e = (Universe.exprs u).1 \/ In e (Universe.exprs u).2.
+    <-> e = (exprs u).1 \/ In e (exprs u).2.
   Proof.
     etransitivity. symmetry. apply UnivExprSet.elements_spec1.
-    pose proof (Universe.exprs_spec' u) as H.
-    destruct (Universe.exprs u) as [e' l]; cbn in *.
+    pose proof (exprs_spec' u) as H.
+    destruct (exprs u) as [e' l]; cbn in *.
     rewrite <- H; clear. etransitivity. apply InA_cons.
     eapply or_iff_compat_l. apply InA_In_eq.
   Qed.
 
-  Lemma In_exprs_rev (u : t0) (e : UnivExpr.t) :
+  Lemma In_exprs_rev (u : t) (e : UnivExpr.t) :
     UnivExprSet.In e u
-    <-> e = (Universe.exprs u).1 \/ In e (List.rev (Universe.exprs u).2).
+    <-> e = (exprs u).1 \/ In e (List.rev (exprs u).2).
   Proof.
     etransitivity. eapply In_exprs.
     apply or_iff_compat_l. apply in_rev.
   Qed.
 
-  Definition map (f : UnivExpr.t -> UnivExpr.t) (u : t0) : t0 :=
+  Definition map (f : UnivExpr.t -> UnivExpr.t) (u : t) : t :=
     let '(e, l) := exprs u in
     add_list (List.map f l) (make' (f e)).
 
@@ -593,15 +625,10 @@ Module Universe.
 
   (** The universe strictly above FOR TYPING (not cumulativity) *)
 
-  Definition super (l : t) : t :=
-    match l with
-    | lSProp => type1
-    | lProp => type1
-    | lType l => lType (map UnivExpr.succ l)
-    end.
+  Definition super (l : t) : t := map UnivExpr.succ l.
 
   (** The l.u.b. of 2 non-prop universe sets *)
-  Program Definition sup0 (u v : t0) : t0 :=
+  Program Definition sup (u v : t) : t :=
     {| t_set := UnivExprSet.union u v |}.
   Next Obligation.
     apply not_Empty_is_empty; intro H.
@@ -612,31 +639,8 @@ Module Universe.
     rewrite t_ne in HH; discriminate.
   Qed.
 
-  Definition sup (u v : t) : t :=
-    match u,v with
-    | lSProp, lProp => lProp
-    | lProp, lSProp => lProp
-    | (lSProp | lProp), u' => u'
-    | u', (lSProp | lProp) => u'
-    | lType l1, lType l2  => lType (sup0 l1 l2)
-    end.
 
-  Definition get_univ_exprs (u : t) (H1 : is_prop u = false) (H2 : is_sprop u = false) : t0.
-  destruct u; try discriminate;easy. Defined.
-
-  (** Type of a product *)
-  Definition sort_of_product (domsort rangsort : t) :=
-    (* Prop and SProp impredicativity *)
-    if Universe.is_prop rangsort || Universe.is_sprop rangsort then rangsort
-    else Universe.sup domsort rangsort.
-
-  Lemma eqb_refl u : eqb u u.
-  Proof.
-    destruct u;auto.
-    now apply UnivExprSet.equal_spec.
-  Qed.
-
-  Lemma elements_not_empty (u : Universe.t0) : UnivExprSet.elements u <> [].
+  Lemma elements_not_empty (u : t) : UnivExprSet.elements u <> [].
   Proof.
     destruct u as [u1 u2]; cbn; intro e.
     unfold UnivExprSet.is_empty, UnivExprSet.elements,
@@ -644,84 +648,39 @@ Module Universe.
     rewrite e in u2; discriminate.
   Qed.
 
-  Definition get_is_level (u : t) : option Level.t :=
-    match u with
-    | lSProp => None
-    | lProp => None
-    | lType l => match UnivExprSet.elements l with
-                 [(l, 0%nat)] => Some l
-               | _ => None
-               end
-    end.
-
-  Global Instance Evaluable' : Evaluable t0
-    := fun v u => let '(e, u) := Universe.exprs u in
+  Global Instance Evaluable' : Evaluable t
+    := fun v u => let '(e, u) := exprs u in
                List.fold_left (fun n e => Nat.max (val v e) n) u (val v e).
-
-  Definition univ_val :=
-    fun v u => match u with
-            | lSProp => USProp
-            | lProp => UProp
-            | lType l => UType (val v l)
-            end.
 
   Lemma val_make' v e
     : val v (make' e) = val v e.
   Proof.
     reflexivity.
   Qed.
-
-  Lemma val_make v l
-    : univ_val v (make l) = UType (val v l).
-  Proof.
-    destruct l; cbnr.
-  Qed.
-
-  Lemma val_make_npl v (l : Level.t)
-    : univ_val v (make l) = UType (val v l).
-  Proof.
-    destruct l; cbnr.
-  Qed.
-
-  Lemma make_inj x y :
-    make x = make y -> x = y.
-  Proof.
-    destruct x, y; try now inversion 1.
-  Qed.
-
-End Universe.
-
-Definition is_propositional u := 
-  Universe.is_prop u || Universe.is_sprop u.
+End UnivLevel.
 
 (** This coercion allows to see the universes as a [UnivExprSet.t] *)
-Coercion Universe.t_set : Universe.t0 >-> UnivExprSet.t.
+Coercion UnivLevel.t_set : UnivLevel.t_ >-> UnivExprSet.t.
 
-Declare Scope univ_scope.
-Delimit Scope univ_scope with u.
-
-Notation "⟦ u ⟧_ v" := (Universe.univ_val v u) (at level 0, format "⟦ u ⟧_ v", v ident) : univ_scope.
+Lemma val_fold_right (u : UnivLevel.t) v :
+  val v u = fold_right (fun e x => Nat.max (val v e) x) (val v (UnivLevel.exprs u).1)
+                       (List.rev (UnivLevel.exprs u).2).
+  Proof.
+  unfold val at 1, UnivLevel.Evaluable'.
+  destruct (UnivLevel.exprs u).
+  now rewrite fold_left_rev_right.
+  Qed.
 
 Ltac u :=
  change LevelSet.elt with Level.t in *;
  change UnivExprSet.elt with UnivExpr.t in *.
  (* change ConstraintSet.elt with UnivConstraint.t in *. *)
 
-
-Lemma val_fold_right (u : Universe.t0) v :
-  val v u = fold_right (fun e x => Nat.max (val v e) x) (val v (Universe.exprs u).1)
-                       (List.rev (Universe.exprs u).2).
-Proof.
-  unfold val at 1, Universe.Evaluable'.
-  destruct (Universe.exprs u).
-  now rewrite fold_left_rev_right.
-Qed.
-
-Lemma val_In_le (u : Universe.t0) v e :
+Lemma val_In_le (u : UnivLevel.t) v e :
   UnivExprSet.In e u -> val v e <= val v u.
 Proof.
   intro H. rewrite val_fold_right.
-  apply Universe.In_exprs_rev in H. destruct (Universe.exprs u); cbn in *.
+  apply UnivLevel.In_exprs_rev in H. destruct (UnivLevel.exprs u); cbn in *.
   clear -H. destruct H as [H|H].
   - subst. induction (List.rev l); cbnr; lia.
   - induction (List.rev l); cbn; invs H.
@@ -729,12 +688,12 @@ Proof.
     + specialize (IHl0 H0). lia.
 Qed.
 
-Lemma val_In_max (u : Universe.t0) v :
+Lemma val_In_max (u : UnivLevel.t) v :
   exists e, UnivExprSet.In e u /\ val v e = val v u.
 Proof.
   eapply iff_ex. {
-    intro. eapply and_iff_compat_r. apply Universe.In_exprs_rev. }
-  rewrite val_fold_right. destruct (Universe.exprs u) as [e l]; cbn in *.
+    intro. eapply and_iff_compat_r. apply UnivLevel.In_exprs_rev. }
+  rewrite val_fold_right. destruct (UnivLevel.exprs u) as [e l]; cbn in *.
   clear. induction (List.rev l); cbn.
   - exists e. split; cbnr. left; reflexivity.
   - destruct IHl0 as [e' [H1 H2]].
@@ -746,15 +705,15 @@ Proof.
       destruct H1 as [H1|H1]; [now left|right]. now constructor 2.
 Qed.
 
-Lemma val_ge_caract (u : Universe.t0) v k :
+Lemma val_ge_caract (u : UnivLevel.t) v k :
   (forall e, UnivExprSet.In e u -> val v e <= k) <-> val v u <= k.
 Proof.
   split.
   - eapply imp_iff_compat_r. {
       eapply iff_forall; intro. eapply imp_iff_compat_r.
-      apply Universe.In_exprs_rev. }
+      apply UnivLevel.In_exprs_rev. }
     rewrite val_fold_right.
-    destruct (Universe.exprs u) as [e l]; cbn; clear.
+    destruct (UnivLevel.exprs u) as [e l]; cbn; clear.
     induction (List.rev l); cbn.
     + intros H. apply H. left; reflexivity.
     + intros H.
@@ -767,14 +726,14 @@ Proof.
   - intros H e He. eapply val_In_le in He. etransitivity; eassumption.
 Qed.
 
-Lemma val_le_caract (u : Universe.t0) v k :
+Lemma val_le_caract (u : UnivLevel.t) v k :
   (exists e, UnivExprSet.In e u /\ k <= val v e) <-> k <= val v u.
 Proof.
   split.
   - eapply imp_iff_compat_r. {
-      eapply iff_ex; intro. eapply and_iff_compat_r. apply Universe.In_exprs_rev. }
+      eapply iff_ex; intro. eapply and_iff_compat_r. apply UnivLevel.In_exprs_rev. }
     rewrite val_fold_right.
-    destruct (Universe.exprs u) as [e l]; cbn; clear.
+    destruct (UnivLevel.exprs u) as [e l]; cbn; clear.
     induction (List.rev l); cbn.
     + intros H. destruct H as [e' [[H1|H1] H2]].
       * now subst.
@@ -790,7 +749,7 @@ Qed.
 
 
 
-Lemma val_caract (u : Universe.t0) v k :
+Lemma val_caract (u : UnivLevel.t) v k :
   val v u = k
   <-> (forall e, UnivExprSet.In e u -> val v e <= k)
     /\ exists e, UnivExprSet.In e u /\ val v e = k.
@@ -807,7 +766,7 @@ Proof.
 Qed.
 
 Lemma val_add v e s
-  : val v (Universe.add e s) = Nat.max (val v e) (val v s).
+  : val v (UnivLevel.add e s) = Nat.max (val v e) (val v s).
 Proof.
   apply val_caract. split.
   - intros e' H. apply UnivExprSet.add_spec in H. destruct H as [H|H].
@@ -820,7 +779,7 @@ Proof.
 Qed.
 
 Lemma val_sup v s1 s2 :
-  val v (Universe.sup0 s1 s2) = Nat.max (val v s1) (val v s2).
+  val v (UnivLevel.sup s1 s2) = Nat.max (val v s1) (val v s2).
 Proof.
   eapply val_caract. cbn. split.
   - intros e' H. eapply UnivExprSet.union_spec in H. destruct H as [H|H].
@@ -841,34 +800,165 @@ Proof.
   apply UnivExprSetFact.for_all_b; proper.
 Qed.
 
-Definition univ_val_max v1 v2 :=
-  match v1, v2 with
-  | UProp, UProp => UProp
-  | USProp, USProp => USProp
-  | UType v, UType v' => UType (Nat.max v v')
-  | _, UType _ => v2
-  | UType _, _ => v1
-  | UProp, USProp => UProp
-  | USProp, UProp => UProp
+
+
+(** * Universes *)
+
+Module Universe.
+  (** A universe combines a sort family with a universe level *)
+  Record t_ := {
+    t_sort : SortFamily.t ;
+    t_level : UnivLevel.t }.
+  Derive NoConfusion for t_.
+
+  Instance t_eqdec : EqDec t_.
+  Proof. eqdec_proof. Qed.
+
+  Definition t := t_.
+
+  (* comparing universe levels even if the sorts might be impredicative
+     otherwise [eqb_true_iff] won't hold *)
+  Definition eqb (u1 u2 : t) : bool :=
+    SortFamily.eqb u1.(t_sort) u2.(t_sort)
+    && UnivLevel.eqb u1.(t_level) u2.(t_level).
+
+  Definition set0 := UnivLevel.make' (UnivExpr.make Level.lSet).
+
+  Definition lType := Build_t_ SortFamily.sfType.
+  Definition lProp := Build_t_ SortFamily.sfProp set0.
+  Definition lSProp := Build_t_ SortFamily.sfSProp set0.
+
+  (** Create a universe representing the given level. *)
+  Definition make (l : Level.t) : t :=
+     lType (UnivLevel.make' (UnivExpr.make l)).
+
+  Definition of_expr e :=
+    (lType (UnivLevel.make' e)).
+
+  Definition add_to_exprs (e : UnivExpr.t) (u : t) : t :=
+    {| t_sort := u.(t_sort) ; t_level := UnivLevel.add e u.(t_level) |}.
+
+  Definition add_list_to_exprs (es : list UnivExpr.t) (u : t) : t :=
+    {| t_sort := u.(t_sort) ; t_level := UnivLevel.add_list es u.(t_level) |}.
+
+  (** Test if the universe is a lub of levels or contains +n's. *)
+  Definition is_levels (u : t) : bool :=
+    UnivLevel.is_levels u.(t_level).
+
+  (** Test if the universe is a level or an algebraic universe. *)
+  Definition is_level (u : t) : bool :=
+    UnivLevel.is_level u.(t_level).
+
+  (* Beware that a sort variable can be instanciated afterwards...*)
+  Definition is_sprop (u : t) : bool :=
+    match u.(t_sort) with
+      | SortFamily.sfSProp => true
+      | _ => false
+    end.
+
+  Definition is_prop (u : t) : bool :=
+    match u.(t_sort) with
+      | SortFamily.sfProp => true
+      | _ => false
+    end.
+
+  Definition is_sort_var (u : t) : bool :=
+    match u.(t_sort) with
+      | SortFamily.sfVar _ => true
+      | _ => false
   end.
 
-Lemma val_universe_sup v u1 u2 :
-  Universe.univ_val v (Universe.sup u1 u2) = univ_val_max (Universe.univ_val v u1) (Universe.univ_val v u2).
+  Definition type0 : t := make Level.lSet.
+  Definition type1 : t := lType (UnivLevel.make' UnivExpr.type1).
+
+
+  (* Used for quoting. *)
+  Definition from_kernel_repr (e : Level.t * bool) (es : list (Level.t * bool)) : t
+    := lType (UnivLevel.add_list (map UnivExpr.from_kernel_repr es)
+                (UnivLevel.make' (UnivExpr.from_kernel_repr e))).
+
+  (** The universe strictly above FOR TYPING (not cumulativity) *)
+
+  (* TODO: is that supposed to be universe in which the sort is living ? *)
+  Definition super (l : t) : t :=
+    lType (UnivLevel.map UnivExpr.succ l.(t_level)).
+
+
+  Definition get_univ_exprs (u : t) : UnivLevel.t := u.(t_level).
+
+  (** Type of a product *)
+  Definition sort_of_product (domsort rangsort : t) :=
+    (* If the sort is impredicative, the actual level is irrelevant *)
+    {| t_sort := rangsort.(t_sort) ;
+       t_level := UnivLevel.sup domsort.(t_level) rangsort.(t_level) |}.
+
+  Lemma eqb_refl u : eqb u u.
+  Proof.
+    apply/andP;split; first apply SortFamily.eqb_refl.
+    now apply UnivExprSet.equal_spec.
+  Qed.
+
+  Definition univ_val : valuation -> t -> universes :=
+    fun v u => (SortFamily.sort_val v u.(t_sort), val v u.(t_level)).
+
+  Definition uType n : universes := (UType, n).
+
+  Lemma val_make v l
+    : univ_val v (make l) = uType (val v l).
+  Proof.
+    destruct l; cbnr.
+  Qed.
+
+  Notation val_make_npl := val_make.
+
+  Lemma make_inj x y :
+    make x = make y -> x = y.
 Proof.
-  destruct u1 as [ | | l1]; destruct u2 as [ | | l2];cbn;try lia; auto.
-  f_equal. apply val_sup.
+    destruct x, y; try now inversion 1.
 Qed.
 
+End Universe.
+
+(* Definition is_propositional u :=  *)
+(*   Universe.is_prop u || Universe.is_sprop u. *)
+
+
+Declare Scope univ_scope.
+Delimit Scope univ_scope with u.
+
+Notation "⟦ u ⟧_ v" := (Universe.univ_val v u) (at level 0, format "⟦ u ⟧_ v", v ident) : univ_scope.
+
+
+
+
+(* Definition univ_val_max v1 v2 := *)
+(*   match v1, v2 with *)
+(*   | UProp, UProp => UProp *)
+(*   | USProp, USProp => USProp *)
+(*   | UType v, UType v' => UType (Nat.max v v') *)
+(*   | _, UType _ => v2 *)
+(*   | UType _, _ => v1 *)
+(*   | UProp, USProp => UProp *)
+(*   | USProp, UProp => UProp *)
+(*   end. *)
+
+(* Lemma val_universe_sup v u1 u2 : *)
+(*   Universe.univ_val v (Universe.sup u1 u2) = univ_val_max (Universe.univ_val v u1) (Universe.univ_val v u2). *)
+(* Proof. *)
+(*   destruct u1 as [ | | l1]; destruct u2 as [ | | l2];cbn;try lia; auto. *)
+(*   f_equal. apply val_sup. *)
+(* Qed. *)
+
 Lemma is_prop_val u :
-  Universe.is_prop u -> forall v, Universe.univ_val v u = UProp.
+  Universe.is_prop u -> forall v, (Universe.univ_val v u).1 = UProp.
 Proof.
-  destruct u as [| | u];try discriminate;auto.
+  move: u => [[]] //.
 Qed.
 
 Lemma is_sprop_val u :
-  Universe.is_sprop u -> forall v, Universe.univ_val v u = USProp.
+  Universe.is_sprop u -> forall v, (Universe.univ_val v u).1 = USProp.
 Proof.
-  destruct u as [| | u];try discriminate;auto.
+  move: u=> [[]] //.
 Qed.
 
 (* 
@@ -887,46 +977,46 @@ Qed. *)
 
 
 Lemma val_is_prop u v :
-  Universe.univ_val v u = UProp <-> Universe.is_prop u.
+  (Universe.univ_val v u).1 = UProp -> Universe.is_prop u \/ Universe.is_sort_var u.
 Proof.
-  destruct u; auto;cbn in *; intuition congruence.
+  move: u=> [[]] //=; dintuition.
 Qed.
 
 Lemma val_is_sprop u v :
-  Universe.univ_val v u = USProp <-> Universe.is_sprop u.
+  (Universe.univ_val v u).1 = USProp -> Universe.is_sprop u \/ Universe.is_sort_var u.
 Proof.
-  destruct u;auto;cbn in *; intuition congruence.
+  move: u=> [[]] //=; dintuition.
 Qed.
 
-Lemma is_prop_and_is_sprop_val_false u :
-  Universe.is_prop u = false -> Universe.is_sprop u = false -> 
-  forall v, ∑ n, Universe.univ_val v u = UType n.
-Proof.
-  intros Hp Hsp v.
-  destruct u; try discriminate. simpl. eexists; eauto.
-Qed.
+(* Lemma is_prop_and_is_sprop_val_false u : *)
+(*   Universe.is_prop u = false -> Universe.is_sprop u = false -> *)
+(*   forall v, ∑ n, Universe.univ_val v u = UType n. *)
+(* Proof. *)
+(*   intros Hp Hsp v. *)
+(*   destruct u; try discriminate. simpl. eexists; eauto. *)
+(* Qed. *)
 
 Lemma val_is_prop_false u v n :
-  Universe.univ_val v u = UType n -> Universe.is_prop u = false.
+  Universe.univ_val v u = Universe.uType n -> Universe.is_prop u = false.
 Proof.
   pose proof (is_prop_val u) as H. destruct (Universe.is_prop u); cbnr.
-  rewrite (H eq_refl v). discriminate.
+  move=>[=]+_;move: (H eq_refl v)=> /= -> //.
 Qed.
 
-Lemma eq_univ (u v : Universe.t0) :
+Lemma eq_univ (u v : UnivLevel.t) :
   u = v :> UnivExprSet.t -> u = v.
 Proof.
   destruct u as [u1 u2], v as [v1 v2]; cbn. intros X; destruct X.
   now rewrite (uip_bool _ _ u2 v2).
 Qed.
 
-Lemma eq_univ' (u v : Universe.t0) :
+Lemma eq_univ' (u v : UnivLevel.t) :
   UnivExprSet.Equal u v -> u = v.
 Proof.
   intro H. now apply eq_univ, UnivExprSet.eq_leibniz.
 Qed.
 
-Lemma eq_univ'' (u v : Universe.t0) :
+Lemma eq_univ'' (u v : UnivLevel.t) :
   UnivExprSet.elements u = UnivExprSet.elements v -> u = v.
 Proof.
   intro H. apply eq_univ.
@@ -935,24 +1025,7 @@ Proof.
   destruct H. now rewrite (uip_bool _ _ u2 v2).
 Qed.
 
-Lemma get_is_level_correct u l :
-  Universe.get_is_level u = Some l -> u = Universe.make l.
-Proof.
-  intro H.
-  destruct u eqn:Hu;cbn in *.
-  - inversion H;subst;reflexivity.
-  - inversion H;subst;reflexivity.
-  - unfold Universe.make.
-    destruct (UnivExprSet.elements _) as [|l0 L] eqn:Hu1; [discriminate|].
-    destruct l0, L; try discriminate.
-    * destruct t,n;inversion H;subst.
-      apply f_equal.
-      apply eq_univ'';unfold UnivExpr.make.
-      cbn. simpl in Hu1. rewrite Hu1. reflexivity.
-    * destruct e,n;inversion H;subst.
-Qed.
-
-Lemma univ_expr_eqb_true_iff (u v : Universe.t0) :
+Lemma univ_expr_eqb_true_iff (u v : UnivLevel.t) :
   UnivExprSet.equal u v <-> u = v.
 Proof.
   split.
@@ -965,9 +1038,8 @@ Lemma eqb_true_iff u v :
   Universe.eqb u v <-> u = v.
 Proof.
   split. 2: intros ->; apply Universe.eqb_refl.
-  intro H.
-  destruct u,v;auto;try discriminate.
-  apply f_equal. now apply univ_expr_eqb_true_iff.
+  destruct u,v=> /=. move=>/andP/=[/SortFamily.eqb_spec Hs Hl].
+  f_equal=> //; now apply univ_expr_eqb_true_iff.
 Qed.
 
 Lemma UnivExprSet_for_all_false f u :
@@ -982,13 +1054,13 @@ Proof.
   right; now rewrite IHl.
 Qed.
 
-Lemma UnivExprSet_For_all_exprs (P : UnivExpr.t -> Prop) (u : Universe.t0)
+Lemma UnivExprSet_For_all_exprs (P : UnivExpr.t -> Prop) (u : UnivLevel.t)
   : UnivExprSet.For_all P u
-    <-> P (Universe.exprs u).1 /\ Forall P (Universe.exprs u).2.
+    <-> P (UnivLevel.exprs u).1 /\ Forall P (UnivLevel.exprs u).2.
 Proof.
   etransitivity.
   - eapply iff_forall; intro e. eapply imp_iff_compat_r.
-    apply Universe.In_exprs.
+    apply UnivLevel.In_exprs.
   - cbn; split.
     + intro H. split. apply H. now left.
       apply Forall_forall. intros x H0.  apply H; now right.
@@ -996,54 +1068,13 @@ Proof.
       eapply Forall_forall in H2; tea.
 Qed.
 
-Lemma sup0_comm x1 x2 :
-  Universe.sup0 x1 x2 = Universe.sup0 x2 x1.
+Lemma sup_comm x1 x2 :
+  UnivLevel.sup x1 x2 = UnivLevel.sup x2 x1.
 Proof.
   apply eq_univ'; simpl. unfold UnivExprSet.Equal.
   intros H. rewrite !UnivExprSet.union_spec. intuition.
 Qed.
 
-Lemma sup_comm x1 x2 :
-  Universe.sup x1 x2 = Universe.sup x2 x1.
-Proof.
-  destruct x1,x2;auto.
-  cbn;apply f_equal;apply sup0_comm.
-Qed.
-
-Lemma is_prop_sort_sup x1 x2 :
-  Universe.is_prop (Universe.sup x1 x2)
-  -> Universe.is_prop x2 \/ Universe.is_sprop x2 .
-Proof. destruct x1,x2;auto. Qed.
-
-Lemma is_prop_sort_sup' x1 x2 :
-  Universe.is_prop (Universe.sup x1 x2)
-  -> Universe.is_prop x1 \/ Universe.is_sprop x1 .
-Proof. destruct x1,x2;auto. Qed.
-
-Lemma is_prop_or_sprop_sort_sup x1 x2 :
-  Universe.is_sprop (Universe.sup x1 x2) -> Universe.is_sprop x2.
-Proof. destruct x1,x2;auto. Qed.
-
-Lemma is_prop_sort_sup_prop x1 x2 :
-  Universe.is_prop x1 && Universe.is_prop x2 ->
-  Universe.is_prop (Universe.sup x1 x2).
-Proof. destruct x1,x2;auto. Qed.
-
-Lemma is_prop_or_sprop_sort_sup_prop x1 x2 :
-  Universe.is_sprop x1 && Universe.is_sprop x2 ->
-  Universe.is_sprop (Universe.sup x1 x2).
-Proof. destruct x1,x2;auto. Qed.
-
-Lemma is_prop_sup u s :
-  Universe.is_prop (Universe.sup u s) ->
-  (Universe.is_prop u \/ Universe.is_sprop u) /\
-  (Universe.is_prop s \/ Universe.is_sprop s).
-Proof. destruct u,s;auto. Qed.
-
-Lemma is_sprop_sup_iff u s :
-  Universe.is_sprop (Universe.sup u s) <->
-  (Universe.is_sprop u /\ Universe.is_sprop s).
-Proof. split;destruct u,s;intuition. Qed.
 
 Lemma is_prop_sort_prod x2 x3 :
   Universe.is_prop (Universe.sort_of_product x2 x3)
@@ -1051,7 +1082,6 @@ Lemma is_prop_sort_prod x2 x3 :
 Proof.
   unfold Universe.sort_of_product.
   destruct x3;cbn;auto.
-  intros;simpl in *;destruct x2;auto.
 Qed.
 
 Lemma is_sprop_sort_prod x2 x3 :
@@ -1060,8 +1090,17 @@ Lemma is_sprop_sort_prod x2 x3 :
 Proof.
   unfold Universe.sort_of_product.
   destruct x3;cbn;auto.
-  intros;simpl in *;destruct x2;auto.
 Qed.
+
+(** * Constraints on sort families *)
+
+Module SortConstraint := PairOrderedType SortFamily SortFamily.
+Module SortConstraintSet := MSetList.Make SortConstraint.
+Module SortConstraintSetFact := WFactsOn SortConstraint SortConstraintSet.
+Module SortConstraintSetProp := WPropertiesOn SortConstraint SortConstraintSet.
+
+(** * Constraints on levels *)
+
 
 Module ConstraintType.
   Inductive t_ : Set := Le (z : Z) | Eq.
